chapter01-basics/demos/demo17.dfy
@@ -1,14 +1,25 @@
 // Recursion
 
 // Let's define a function, and export properties of it with an ensures.
+/*
 function Evens(count:int) : (outseq:seq<int>)
   ensures forall idx :: 0<=idx<|outseq| ==> outseq[idx] == 2 * idx
 {
   if count==0 then [] else Evens(count) + [2 * (count-1)]
 }
+*/
+
+function EvensOk(count:int) : (outseq:seq<int>)
+  requires 0 <= count
+  ensures count == |outseq|
+  ensures forall idx :: 0<=idx<|outseq| ==> outseq[idx] == 2 * idx
+{
+  var outseq := if count==0 then [] else EvensOk(count - 1) + [2 * (count-1)];
+  outseq
+}
 
 // Walk through this sequence
-
+/*
 Error: cannot prove termination; try supplying a decreases clause
 
 Try adding 'decreases count'.
@@ -33,3 +44,5 @@ Turns out you can insert assertions before the expression in a function.
 Let's use a var (let) expression to put outseq in scope.
 
 Punchline: it doesn't know |outseq|==count
+
+*/
