chapter01-basics/exercises/exercise04.dfy
@@ -25,5 +25,5 @@ lemma TheseTwoPredicatesAreEquivalent(x:int, y:int)
 // Add a precondition to make this lemma verify.
 lemma FourTimesIsPrettyBig(x:int)
 {
-  assert AtLeastTwiceAsBigPredicate(Double(Double(x)), x);
+  assert x == 0 ==> AtLeastTwiceAsBigPredicate(Double(Double(x)), x);
 }
