chapter01-basics/exercises/exercise06.dfy
@@ -24,6 +24,6 @@ lemma SomeAssertionsAboutSets()
   // |x| on a set is cardinality.
   // (set<T> is always finite; there is another type iset<T> for
   // possibly-infinite sets.)
-  assert |happySet| == 7;
+  assert |happySet| == 6;
 }
 
