chapter01-basics/exercises/exercise11.dfy
@@ -5,8 +5,11 @@
 // so there are 9 TextAlign instances (all combinations).
 // Note that it's okay to omit the parens for zero-element constructors.
 datatype HAlign = Left | Center | Right
+// 3
 datatype VAlign = Top | Middle | Bottom
+// 3
 datatype TextAlign = TextAlign(hAlign:HAlign, vAlign:VAlign)
+// 9
 
 // If you squint, you'll believe that unions are like
 // sums. There's one "Top", one "Middle", and one "Bottom"
@@ -14,8 +17,10 @@ datatype TextAlign = TextAlign(hAlign:HAlign, vAlign:VAlign)
 
 // There are two instances of GraphicsAlign
 datatype GraphicsAlign = Square | Round
+// 2
 
 // So if we make another tagged-union (sum) of TextAlign or GraphicsAlign,
 // it has how many instances?
 // (That's the exercise, to answer that question. No Dafny required.)
 datatype PageElement = Text(ta:TextAlign) | Graphics(ga:GraphicsAlign)
+// 11
