chapter01-basics/exercises/exercise19.dfy
@@ -9,8 +9,8 @@ method FindMax(intSeq:seq<int>) returns (maxIndex:nat)
     var count:nat := 0;
     maxIndex := 0;
     while(count < |intSeq|)
-        invariant true
-        invariant true
+        invariant maxIndex<|intSeq|
+        invariant forall idx:nat | idx<count && idx < |intSeq| :: intSeq[idx] <= intSeq[maxIndex]
         invariant true
     {
         if(intSeq[maxIndex] < intSeq[count]) {
